simplify 2

sort/simplest01.v
@@ -3,227 +3,179 @@ Import ListNotations.
 From mathcomp Require Import ssreflect ssrnat ssrbool eqtype.
 
 
-Fixpoint slide (i:nat) (l:list nat) :=
-  match l with
-  | [] => (i, [])
-  | h :: t => 
-    if i < h then 
-      match slide h t with (h', t') => (h', i :: t') end
-    else 
-      match slide i t with (i', t') => (i', h :: t') end
-  end.
+Section GeneralLemmas.
+  Lemma indep_prod : forall (A B C:Type) (f:A -> B -> C) (ab:A*B),
+    (let (a, b) := ab in (f a b)) = f (fst ab) (snd ab).
+  Proof. intuition. Qed.
 
-Lemma indep_prod : forall (A B C:Type) (f:A -> B -> C) (ab:A*B),
-  (let (a, b) := ab in (f a b)) = f (fst ab) (snd ab).
-Proof. intuition. Qed.
-
-Lemma slide_hold_length : forall i l, 
-  length l = length (snd (slide i l)).
-Proof.
-  move=> i l. move:i. induction l. done.
-  move=> i. rewrite /= 2!indep_prod. 
-  case H : (i < a) => /=; apply f_equal, IHl.
-Qed.
-
-Inductive sorted : list nat -> Prop :=
-| sorted_nil : sorted []
-| sorted_1 : forall x, sorted [x]
-| sorted_cons : forall x y l,
-    x <= y -> sorted (y :: l) -> sorted (x :: y :: l).
-
-Lemma cons_sorted : forall h t, sorted (h :: t) -> sorted t.
-Proof. move=> h [|i l] S. apply sorted_nil. inversion S. apply H3. Qed.
-
-Lemma cons_cons_sorted : forall a h t, 
-  sorted (a :: h :: t) -> sorted (a :: t).
-Proof.
-  move=> a h [|h2 t'] S. apply sorted_1. inversion S. inversion H3.
-  apply (sorted_cons _ _ _ (leq_trans H1 H6) H8).
-Qed.
-
-Lemma leq_lt : forall n m, (n < m) = false -> n <= m -> n = m.
-Proof. 
-  move=> n m. rewrite ltnNge. move/eqP/eqP => Nlt Hle.
-  apply/eqP. rewrite eqn_leq. apply /andP; apply conj.
-  apply Hle. apply Nlt.
-Qed.
-
-Lemma slide_cons : forall a l, sorted (a :: l) ->
-  a :: l = (let (a', l') := slide a l in (l' ++ [a'])).
-Proof.
-  move=>a l. move: a. induction l; move=> /= a0 S. done.
-  rewrite 3!indep_prod /=. case H: (a0 < a) => /=.
-  - apply f_equal. inversion S.
-    by rewrite (IHl _ H4) indep_prod.
-  - inversion S. case (leq_lt _ _ H H2). apply f_equal.
-    rewrite IHl. by rewrite indep_prod.
-    apply (cons_cons_sorted _ _ _ S).
-Qed.
-
-Lemma leq_all_cons_sorted' : forall a i l, 
-  sorted (a :: l) -> a <= i -> 
-  sorted (let (h, t) := slide i l in t ++ [h]) ->
-  sorted (let (h, t) := slide i l in a :: t ++ [h]).
-Proof.
-  move=> a i [|h t] S Hle /=.
-  - apply sorted_cons, Hle.
-  - rewrite 4!indep_prod; case H: (i < h) => S2 /=.
-    apply (sorted_cons _ _ _ Hle), S2.
-    inversion S. apply (sorted_cons _ _ _ H2 S2).
-Qed.
-
-Lemma slide_sorted' : forall a l, sorted l -> 
-  sorted (let (h, t) := slide a l in t ++ [h]).
-Proof.
-  fix slide_sorted' 2.
-  move=> a [|h t] S /=. apply sorted_1. case H: (a < h); rewrite 2!indep_prod /=;
-  rewrite -(indep_prod _ _ _ (fun w1 w2 => _ :: w2 ++ [w1])); apply leq_all_cons_sorted'.
-  - apply (cons_cons_sorted _ h _), (fun Hw => sorted_cons _ _ _ Hw S), ltnW, H.  
-  - apply ltnW, H.
-  - apply slide_sorted', (cons_sorted _ _ S).
-  - apply S.
-  - move:H. rewrite ltnNge. by move/eqP/eqP.
-  - apply slide_sorted', (cons_sorted _ _ S).
-Qed.
-
-Corollary leq_all_cons_sorted : forall a i l, 
-  sorted (a :: l) -> a <= i -> 
-  sorted (let (h, t) := slide i l in a :: t ++ [h]).
-Proof.
-  move=> a i l S Hle. apply leq_all_cons_sorted'. apply S. apply Hle.
-  apply slide_sorted'. apply (cons_sorted _ _ S).
-Qed.
-
-Lemma app_cons_comm : forall A (l1:list A) n l2, 
+  Lemma leq_lt : forall {n m}, (n < m) = false -> n <= m -> n = m.
+  Proof. 
+    move=> n m. rewrite ltnNge. move/eqP/eqP => Nlt Hle.
+    apply/eqP. rewrite eqn_leq. apply /andP; apply conj.
+    apply Hle. apply Nlt.
+  Qed.
+  
+  Lemma app_cons_comm : forall A (l1:list A) n l2, 
   l1 ++ n :: l2 = (l1 ++ [n]) ++ l2.
-Proof. induction l1; by [|move=>n l2; rewrite -3!app_comm_cons IHl1]. Qed.
+  Proof. induction l1; by [|move=>n l2; rewrite -3!app_comm_cons IHl1]. Qed.
+End GeneralLemmas.
 
-Lemma sorted_snoc : forall l n, sorted (l ++ [n]) -> sorted l.
-Proof.
-  induction l; intros n S. apply sorted_nil. rewrite -app_comm_cons in S.
-  induction l. apply sorted_1. inversion S. apply sorted_cons. apply H1.
-  apply cons_sorted in S. apply (IHl _ S).
-Qed.
+Section Sorted.
+  Inductive sorted : list nat -> Prop :=
+  | sorted_nil : sorted []
+  | sorted_1 : forall x, sorted [x]
+  | sorted_cons : forall {x y l},
+      x <= y -> sorted (y :: l) -> sorted (x :: y :: l).
 
-Lemma app_sorted : forall l1 l2, sorted (l1 ++ l2) -> sorted l1.
-Proof.
-  move=> l1 l2. move:l1. induction l2; move=> l1. by rewrite app_nil_r.
-  rewrite app_cons_comm => S. apply IHl2 in S.
-  by apply sorted_snoc in S.
-Qed.
+  Lemma sorted_tail : forall {h t}, sorted (h :: t) -> sorted t.
+  Proof. move=> h [|i l] S. apply sorted_nil. inversion S. apply H3. Qed.
 
-Corollary leq_all_cons_sorted_snd : forall a i l,
-  sorted (a :: l) -> a <= i -> sorted (a :: snd (slide i l)).
-Proof.
-  move=> a i l S Hle. move: (leq_all_cons_sorted _ _ _ S Hle).
-  rewrite indep_prod app_comm_cons. apply app_sorted.
-Qed.
+  Lemma sorted_1_3toend : forall {a h t}, 
+    sorted (a :: h :: t) -> sorted (a :: t).
+  Proof.
+    move=> a h [|h2 t'] S. apply sorted_1. inversion S. inversion H3.
+    apply (sorted_cons (leq_trans H1 H6) H8).
+  Qed.
+(* 
+  Lemma sorted_before_cons : forall l n, sorted (l ++ [n]) -> sorted l.
+  Proof.
+    induction l; intros n S. apply sorted_nil. rewrite -app_comm_cons in S.
+    induction l. apply sorted_1. inversion S. apply sorted_cons. apply H1.
+    apply sorted_tail in S. apply (IHl _ S).
+  Qed.
 
-Lemma sorted_trans_app_app: forall l1 h t l3,
-  sorted (l1 ++ h :: t) -> sorted (h :: t ++ l3) -> sorted (l1 ++ h :: t ++ l3).
-Proof.
-  induction l1. done.
-  destruct l1.
-  - move=> /= h t l3 S1 S2. apply sorted_cons. 
-    inversion S1. apply H1. apply S2.
-  - move:IHl1 => /= IHl1 h t l3 S1 S2. inversion S1.
-    apply sorted_cons. apply H1. apply IHl1. apply H3. apply S2.
-Qed.
+  Lemma sorted_before_app : forall l1 l2, sorted (l1 ++ l2) -> sorted l1.
+  Proof.
+    move=> l1 l2. move:l1. induction l2; move=> l1. by rewrite app_nil_r.
+    rewrite app_cons_comm => S. apply IHl2 in S.
+    by apply sorted_before_cons in S.
+  Qed. *)
+End Sorted.
 
-Lemma slide_leq : forall i l, i <= fst (slide i l).
-Proof.
-  fix slide_leq 2.
-  move => i [|h t] => /=. done. 
-  case H: (i < h); rewrite indep_prod /=.
-  - apply (leq_trans (n := h)). apply ltnW, H. apply slide_leq.
-  - apply slide_leq.
-Qed.
+Section Slide.
+  Fixpoint slide (i:nat) (l:list nat) :=
+    match l with
+    | [] => (i, [])
+    | h :: t => 
+      if i < h then 
+        match slide h t with (h', t') => (h', i :: t') end
+      else 
+        match slide i t with (i', t') => (i', h :: t') end
+    end.
 
-Lemma leq_fst_slide : forall a n l, a <= n ->
-  fst (slide a (n :: l)) = fst (slide n l).
-Proof.
-  move=> a n l Hle => /=. case H: (a < n); rewrite indep_prod /=.
-  done. by case (leq_lt _ _ H Hle).
-Qed.
+  Lemma slide_cons_fst_comm : forall i n l,
+    slide i (n :: l) = slide n (i :: l).
+  Proof.
+    move=> i n l. rewrite /= 2!indep_prod /=. 
+    case H: (i < n); case H2: (n < i).
+    - pose (ltn_geF H). apply ltnW in H2. by rewrite e in H2.
+    - done.
+    - done.
+    - rewrite ltnNge in H2. move:H2. move/eqP/eqP => H2.
+      by case (leq_lt H H2).
+  Qed.
 
-Lemma leq_snd_slide : forall a n l, a <= n ->
-  snd (slide a (n :: l)) = a :: snd (slide n l).
-Proof.
-  move=> a n l Hle => /=. case H: (a < n); rewrite indep_prod /=.
-  done. by case (leq_lt _ _ H Hle).
-Qed.
+  Lemma slide_hold_length : forall i l, 
+    length l = length (snd (slide i l)).
+  Proof.
+    move=> i l. move:i. induction l. done.
+    move=> i. rewrite /= 2!indep_prod. 
+    case H : (i < a) => /=; apply f_equal, IHl.
+  Qed.
 
-Lemma slide_cons_fst_comm : forall i n l,
-  slide i (n :: l) = slide n (i :: l).
-Proof.
-  move=> i n l. rewrite /= 2!indep_prod /=. 
-  case H: (i < n); case H2: (n < i).
-  - pose (ltn_geF H). apply ltnW in H2. by rewrite e in H2.
-  - done.
-  - done.
-  - rewrite ltnNge in H2. move:H2. move/eqP/eqP => H2.
-    by case (leq_lt _ _ H H2).
-Qed.
+  Lemma slide_hold_sortedlist : forall a l, sorted (a :: l) ->
+    a :: l = (let (a', l') := slide a l in (l' ++ [a'])).
+  Proof.
+    move=>a l. move: a. induction l; move=> /= a0 S. done.
+    rewrite 3!indep_prod /=. case H: (a0 < a) => /=.
+    - apply f_equal. inversion S.
+      by rewrite (IHl _ H4) indep_prod.
+    - inversion S. case (leq_lt H H2). apply f_equal.
+      rewrite IHl. by rewrite indep_prod.
+      apply (sorted_1_3toend S).
+  Qed.
 
-Lemma slide_geq_sorted : forall i l j, sorted l ->
-  let (i', l') := slide i l in (i' <= j -> sorted (l' ++ [j])).
-Proof.
-  move=> i l j. rewrite indep_prod. move: l i j. induction l.
-  move=> i j S Hle; apply sorted_1.
-  move=> i j S /=. rewrite 2! indep_prod. 
-  destruct l; rewrite /=.
-  - case H: (i < a) => /= Hle; apply sorted_cons; try apply sorted_1.
-    - apply (leq_trans(n:=a)). apply ltnW, H. apply Hle.
-    - apply (leq_trans(n:=i)). move:H. rewrite ltnNge. 
-      by move/eqP/eqP. apply Hle.
-  - inversion S. case Hc: (i < a).
-    - case Hc2: (a < n); rewrite indep_prod /= => Hle.
+  Lemma index_leq_fstslide : forall i l, i <= fst (slide i l).
+  Proof.
+    fix index_leq_fstslide 2.
+    move => i [|h t] => /=. done. 
+    case H: (i < h); rewrite indep_prod /=.
+    - apply (leq_trans (n := h)). apply ltnW, H. apply index_leq_fstslide.
+    - apply index_leq_fstslide.
+  Qed.
+
+  Lemma leq_simpl_fstslide : forall {a n l}, a <= n ->
+    fst (slide a (n :: l)) = fst (slide n l).
+  Proof.
+    move=> a n l Hle => /=. case H: (a < n); rewrite indep_prod /=.
+    done. by case (leq_lt H Hle).
+  Qed.
+
+  Lemma leq_simpl_sndslide : forall {a n l}, a <= n ->
+    snd (slide a (n :: l)) = a :: snd (slide n l).
+  Proof.
+    move=> a n l Hle => /=. case H: (a < n); rewrite indep_prod /=.
+    done. by case (leq_lt H Hle).
+  Qed.
+
+  Lemma sorted_slide_snoc_geqind : forall i l j, sorted l ->
+    let (i', l') := slide i l in (i' <= j -> sorted (l' ++ [j])).
+  Proof.
+    move=> i l j. rewrite indep_prod. move: l i j. induction l.
+    move=> i j S Hle; apply sorted_1.
+    move=> i j S /=. rewrite 2! indep_prod. 
+    destruct l; rewrite /=.
+    - case H: (i < a) => /= Hle; apply sorted_cons; try apply sorted_1.
+      - apply (leq_trans(n:=a)). apply ltnW, H. apply Hle.
+      - apply (leq_trans(n:=i)). move:H. rewrite ltnNge. 
+        by move/eqP/eqP. apply Hle.
+    - inversion S. case Hc: (i < a); [case Hc2: (a < n) | case Hc2: (i < n)]; 
+      rewrite indep_prod /= => Hle.
       - apply sorted_cons. apply ltnW, Hc.
-        rewrite app_comm_cons -(leq_snd_slide _ _ _ H1).
-        apply IHl. done. by rewrite (leq_fst_slide _ _ _ H1).
-      - move:IHl H3. case (leq_lt _ _ Hc2 H1) => IHl H3.
+        rewrite app_comm_cons -(leq_simpl_sndslide H1).
+        apply IHl. done. by rewrite (leq_simpl_fstslide H1).
+      - move:IHl H3. case (leq_lt Hc2 H1) => IHl H3.
         apply sorted_cons. apply ltnW, Hc. 
-        rewrite app_comm_cons -(leq_snd_slide _ _ _ (leqnn _)).
-        apply IHl. done. by rewrite (leq_fst_slide _ _ _ (leqnn _)).
-    - case Hc2: (i < n); rewrite indep_prod /= => Hle.
+        rewrite app_comm_cons -(leq_simpl_sndslide (leqnn _)).
+        apply IHl. done. by rewrite (leq_simpl_fstslide (leqnn _)).
       - apply sorted_cons. move:Hc. rewrite ltnNge. by move/eqP/eqP.
-        rewrite app_comm_cons -(leq_snd_slide _ _ _ (ltnW Hc2)).
+        rewrite app_comm_cons -(leq_simpl_sndslide (ltnW Hc2)).
         apply IHl. done. 
-        by rewrite (leq_fst_slide _ _ _ (ltnW Hc2)).
+        by rewrite (leq_simpl_fstslide (ltnW Hc2)).
       - apply sorted_cons. apply H1. assert (n <= i) as Hc3. 
         { move:Hc2. rewrite ltnNge. by move/eqP/eqP. }
-        rewrite app_comm_cons -(leq_snd_slide _ _ _ Hc3) slide_cons_fst_comm.
+        rewrite app_comm_cons -(leq_simpl_sndslide Hc3) slide_cons_fst_comm.
         apply IHl. done.
-        by rewrite slide_cons_fst_comm (leq_fst_slide _ _ _ Hc3).
-Qed.
+        by rewrite slide_cons_fst_comm (leq_simpl_fstslide Hc3).
+  Qed.
+End Slide.
 
-Definition slidefb l1 h t :=
-  match slide h l1 with (i, l1') =>
-    match slide i t with (i', l2') => (l1' ++ [i'], l2') end
-  end.
+Section Sort.
+  Definition slidefb l1 h t :=
+    match slide h l1 with (i, l1') =>
+      match slide i t with (i', l2') => (l1' ++ [i'], l2') end
+    end.
 
-Program Definition sort'_noyau (l1: {l | sorted l}) h t 
-  : {l | sorted l} * list nat := slidefb l1 h t.
-Obligation 1.
-  rewrite /slidefb 2!indep_prod /=.
-  move: (slide_geq_sorted h l1 (fst (slide (fst (slide h l1)) t)) H).
-  rewrite indep_prod. apply. apply slide_leq.
-Qed.
+  Program Fixpoint sort_kernel (l1: {l | sorted l}) l2
+      {measure (length l2)} : {l | sorted l} * list nat :=
+    match l2 with
+    | [] => (l1, [])
+    | h :: t => match slidefb l1 h t with
+      (l1s', l2') => sort_kernel l1s' l2' end
+    end.
+  Obligation 1.
+    move: (sorted_slide_snoc_geqind h l1 (fst (slide (fst (slide h l1)) t)) H).
+    rewrite /slidefb 2!indep_prod in Heq_anonymous. inversion Heq_anonymous.
+    rewrite indep_prod. apply. apply index_leq_fstslide.
+  Qed.
+  Obligation 2.
+    rewrite /slidefb 2!indep_prod in Heq_anonymous. inversion Heq_anonymous.
+    by rewrite -slide_hold_length.
+  Qed.
 
-Program Fixpoint sort' (l1s: {l | sorted l}) l2
-    {measure (length l2)} : {l | sorted l} * list nat :=
-  match l2 with
-  | [] => (l1s, [])
-  | h :: t => match sort'_noyau l1s h t with
-    (l1s', l2') => sort' l1s' l2' end
-  end.
-Obligation 1.
-  move:H sort' => /= H sort'.
-  by rewrite /slidefb 2!indep_prod /= -slide_hold_length.
-Qed.
-
-Definition sort (l:list nat) := (proj1_sig (fst (sort' (exist _ nil sorted_nil) l))).
- 
-Goal sort [3; 1; 4; 1; 5; 9; 2; 6; 5; 3; 5]
-  = [1; 1; 2; 3; 3; 4; 5; 5; 5; 6; 9].
-Proof. by compute. Qed.
+  Definition sort (l:list nat) := (proj1_sig (fst (sort_kernel (exist _ nil sorted_nil) l))).
+  
+  Goal sort [3; 1; 4; 1; 5; 9; 2; 6; 5; 3; 5]
+    = [1; 1; 2; 3; 3; 4; 5; 5; 5; 6; 9].
+  Proof. by compute. Qed.
+End Sort.
